Point Inverse

code/ecdsap256/Hacl.Impl.P256.PointInverse.fst
@@ -15,26 +15,44 @@ open Spec.P256.Definitions
 open Hacl.Spec.P256.Felem
 open Spec.P256.MontgomeryMultiplication
 
+open FStar.Mul 
 
-val point_inv: p: point -> result: point -> tempBuffer: lbuffer uint64 (size 88) -> Stack unit
-  (requires fun h -> live h p /\ live h tempBuffer /\ live h result /\
-    disjoint p tempBuffer /\ disjoint result tempBuffer /\
-    eq_or_disjoint p result /\
-    as_nat h (gsub p (size 8) (size 4)) < prime /\ 
-    as_nat h (gsub p (size 0) (size 4)) < prime /\ 
-    as_nat h (gsub p (size 4) (size 4)) < prime)
-  (ensures fun h0 _ h1 -> modifies (loc tempBuffer |+| loc result)  h0 h1 /\  
-    as_nat h1 (gsub result (size 8) (size 4)) < prime /\ 
-    as_nat h1 (gsub result (size 0) (size 4)) < prime /\ 
-    as_nat h1 (gsub result (size 4) (size 4)) < prime /\
-    (
-      let x, y, z = gsub p (size 0) (size 4),  gsub p (size 4) (size 4), gsub p (size 8) (size 4) in 
-      let x3, y3, z3 = gsub result (size 0) (size 4), gsub result (size 4) (size 4), gsub result (size 8) (size 4) in 
-      
-      let xD, yD, zD = fromDomain_ (as_nat h0 x), fromDomain_ (as_nat h0 y), fromDomain_ (as_nat h0 z) in 
-      let x3D, y3D, z3D = fromDomain_ (as_nat h1 x3), fromDomain_ (as_nat h1 y3), fromDomain_ (as_nat h1 z3) in
-      
-      let xN, yN, zN = _point_inverse (xD, yD, zD) in 
-      x3D == xN /\ y3D == yN /\ z3D == zN
-  )
-) 
+
+#set-options "--fuel 0 --ifuel 0 --z3rlimit 200"
+
+val copyH: a: felem -> b: felem -> Stack unit 
+  (requires fun h -> live h a /\ live h b)
+  (ensures fun h0 _ h1 -> modifies (loc b) h0 h1 /\ as_nat h1 b == as_nat h0 a /\ 
+    fromDomain_ (as_nat h1 b) == fromDomain_ (as_nat h0 a))
+
+let copyH a b = 
+  assert_norm (pow2 64 * pow2 64 == pow2 128);
+  assert_norm (pow2 64 * pow2 64 * pow2 64 == pow2 192);
+  assert_norm (pow2 64 * pow2 64 * pow2 64 * pow2 64 == pow2 256);
+
+  let a0 = index a (size 0) in 
+  let a1 = index a (size 1) in 
+  let a2 = index a (size 2) in 
+  let a3 = index a (size 3) in 
+  
+  upd b (size 0) a0;
+  upd b (size 1) a1;
+  upd b (size 2) a2;
+  upd b (size 3) a3
+
+
+
+let point_inv p result tempBuffer = 
+  let h0 = ST.get() in 
+  
+  let temp4 = sub tempBuffer (size 0) (size 4) in 
+  let yP = sub p (size 4) (size 4) in 
+  let yResult = sub result (size 4) (size 4) in 
+
+  Hacl.Impl.P256.LowLevel.PrimeSpecific.p256_sub_zero yP yResult temp4;
+  copyH (sub p (size 0) (size 4)) (sub result (size 0) (size 4)); 
+  copyH (sub p (size 8) (size 4)) (sub result (size 8) (size 4));
+
+  let h1 = ST.get() in 
+  lemmaFromDomain 0;
+  FStar.Math.Lemmas.small_mod 0 prime256
